KeyManagement/Messages.v
@@ -1,9 +1,9 @@
 (* module that takes access type, either KeyId or Permission *)
 
 (* Labels for the labeled transition system, a wrapper for messages *)
-Inductive label  {A} : Type :=
-  Silent : label
-| Action :  A -> label
+Inductive label  {A} {B} : Type :=
+  Silent : A -> label
+| Action : B -> label
 .
 
 Inductive type : Set :=
