KeyManagement/Simulation.v
@@ -23,10 +23,10 @@ Import IdealWorld.IdealNotations
 Set Implicit Arguments.
 
 Definition rstepSilent {A B : Type} (U1 U2 : RealWorld.universe A B) :=
-  RealWorld.step_universe U1 Messages.Silent U2.
+  RealWorld.step_universe U1 RealWorld.silent U2.
 
 Definition istepSilent {A : Type} (U1 U2 : IdealWorld.universe A) :=
-  IdealWorld.lstep_universe U1 Messages.Silent U2.
+  IdealWorld.lstep_universe U1 IdealWorld.silent U2.
 
 Inductive chan_key : Set :=
 | Public (ch_id : IdealWorld.channel_id)
@@ -253,181 +253,180 @@ Definition adv_universe_ok {A B} (U : RealWorld.universe A B) : Prop :=
 Section OperationalSemanticsPredicates.
   Import RealWorld.
 
-  Inductive honest_party_step : forall A B C, rlabel -> option user_id -> data_step0 A B C -> data_step0 A B C -> Prop :=
+  (* Inductive honest_party_step : forall A B C, rlabel -> option user_id -> data_step0 A B C -> data_step0 A B C -> Prop := *)
 
-  (* Plumbing *)
-  | HonestBindRecur : forall {B r r'} (usrs usrs' : honest_users r') (adv adv' : user_data B)
-                      lbl u_id cs cs' qmsgs qmsgs' gks gks' ks ks' mycs mycs' froms froms' sents sents' cur_n cur_n'
-                      (cmd1 cmd1' : user_cmd r) (cmd2 : r -> user_cmd r'),
-      honest_party_step lbl u_id
-                (usrs, adv, cs, gks, ks, qmsgs, mycs, froms, sents, cur_n, cmd1)
-                (usrs', adv', cs', gks', ks', qmsgs', mycs', froms', sents', cur_n', cmd1')
-      -> honest_party_step lbl u_id
-                  (usrs, adv, cs, gks, ks, qmsgs, mycs, froms, sents, cur_n, Bind cmd1 cmd2)
-                  (usrs', adv', cs', gks', ks', qmsgs', mycs', froms', sents', cur_n', Bind cmd1' cmd2)
-  | HonestBindProceed : forall {B r r'} (usrs : honest_users r) (adv : user_data B) cs u_id gks ks qmsgs mycs froms sents cur_n
-                        (v : r') (cmd : r' -> user_cmd r),
-      honest_party_step Silent u_id
-                (usrs, adv, cs, gks, ks, qmsgs, mycs, froms, sents, cur_n, Bind (Return v) cmd)
-                (usrs, adv, cs, gks, ks, qmsgs, mycs, froms, sents, cur_n, cmd v)
+  (* (* Plumbing *) *)
+  (* | HonestBindRecur : forall {B r r'} (usrs usrs' : honest_users r') (adv adv' : user_data B) *)
+  (*                     lbl u_id cs cs' qmsgs qmsgs' gks gks' ks ks' mycs mycs' froms froms' sents sents' cur_n cur_n' *)
+  (*                     (cmd1 cmd1' : user_cmd r) (cmd2 : r -> user_cmd r'), *)
+  (*     honest_party_step lbl u_id *)
+  (*               (usrs, adv, cs, gks, ks, qmsgs, mycs, froms, sents, cur_n, cmd1) *)
+  (*               (usrs', adv', cs', gks', ks', qmsgs', mycs', froms', sents', cur_n', cmd1') *)
+  (*     -> honest_party_step lbl u_id *)
+  (*                 (usrs, adv, cs, gks, ks, qmsgs, mycs, froms, sents, cur_n, Bind cmd1 cmd2) *)
+  (*                 (usrs', adv', cs', gks', ks', qmsgs', mycs', froms', sents', cur_n', Bind cmd1' cmd2) *)
+  (* | HonestBindProceed : forall {B r r'} (usrs : honest_users r) (adv : user_data B) cs u_id gks ks qmsgs mycs froms sents cur_n *)
+  (*                       (v : r') (cmd : r' -> user_cmd r), *)
+  (*     honest_party_step Silent u_id *)
+  (*               (usrs, adv, cs, gks, ks, qmsgs, mycs, froms, sents, cur_n, Bind (Return v) cmd) *)
+  (*               (usrs, adv, cs, gks, ks, qmsgs, mycs, froms, sents, cur_n, cmd v) *)
 
-  | HonestGen : forall {A B} (usrs : honest_users A) (adv : user_data B) cs u_id gks ks qmsgs mycs froms sents cur_n n,
-      honest_party_step Silent u_id (usrs, adv, cs, gks, ks, qmsgs, mycs, froms, sents, cur_n, Gen)
-                (usrs, adv, cs, gks, ks, qmsgs, mycs, froms, sents, cur_n, Return n)
+  (* | HonestGen : forall {A B} (usrs : honest_users A) (adv : user_data B) cs u_id gks ks qmsgs mycs froms sents cur_n n, *)
+  (*     honest_party_step Silent u_id (usrs, adv, cs, gks, ks, qmsgs, mycs, froms, sents, cur_n, Gen) *)
+  (*               (usrs, adv, cs, gks, ks, qmsgs, mycs, froms, sents, cur_n, Return n) *)
 
-  (* Comms  *)
-  | HonestRecv : forall {A B} {t} (usrs : honest_users A) (adv : user_data B) cs u_id gks ks ks' qmsgs qmsgs' mycs mycs' froms froms'
-                 sents cur_n (msg : crypto t) msgs pat newkeys newcs,
-      qmsgs = (existT _ _ msg) :: msgs (* we have a message waiting for us! *)
-      -> qmsgs' = msgs
-      -> findKeysCrypto cs msg = newkeys
-      -> newcs = findCiphers msg
-      -> ks' = ks $k++ newkeys
-      -> mycs' = newcs ++ mycs
-      -> froms' = updateTrackedNonce u_id froms cs msg
-      -> msg_accepted_by_pattern cs u_id pat msg
-      -> honest_party_step (Action (Input msg pat froms)) u_id
-                  (usrs, adv, cs, gks, ks , qmsgs , mycs, froms, sents, cur_n,  Recv pat)
-                  (usrs, adv, cs, gks, ks', qmsgs', mycs', froms', sents, cur_n, Return msg)
+  (* (* Comms  *) *)
+  (* | HonestRecv : forall {A B} {t} (usrs : honest_users A) (adv : user_data B) cs u_id gks ks ks' qmsgs qmsgs' mycs mycs' froms froms' *)
+  (*                sents cur_n (msg : crypto t) msgs pat newkeys newcs, *)
+  (*     qmsgs = (existT _ _ msg) :: msgs (* we have a message waiting for us! *) *)
+  (*     -> qmsgs' = msgs *)
+  (*     -> findKeysCrypto cs msg = newkeys *)
+  (*     -> newcs = findCiphers msg *)
+  (*     -> ks' = ks $k++ newkeys *)
+  (*     -> mycs' = newcs ++ mycs *)
+  (*     -> froms' = updateTrackedNonce u_id froms cs msg *)
+  (*     -> msg_accepted_by_pattern cs u_id pat msg *)
+  (*     -> honest_party_step (Action (Input msg pat froms)) u_id *)
+  (*                 (usrs, adv, cs, gks, ks , qmsgs , mycs, froms, sents, cur_n,  Recv pat) *)
+  (*                 (usrs, adv, cs, gks, ks', qmsgs', mycs', froms', sents, cur_n, Return msg) *)
 
-  | HonestRecvDrop : forall {A B} {t} (usrs : honest_users A) (adv : user_data B) cs suid gks ks qmsgs qmsgs'
-                     mycs froms froms' sents cur_n (msg : crypto t) pat msgs,
-      qmsgs = (existT _ _ msg) :: msgs (* we have a message waiting for us! *)
-      -> qmsgs' = msgs
-      -> froms' = (if msg_signed_addressed (findUserKeys usrs) cs suid msg
-                  then updateTrackedNonce suid froms cs msg
-                  else froms)
-      -> ~ msg_accepted_by_pattern cs suid pat msg
-      -> honest_party_step Silent suid (* Error label ... *)
-                  (usrs, adv, cs, gks, ks, qmsgs , mycs, froms,  sents, cur_n, Recv pat)
-                  (usrs, adv, cs, gks, ks, qmsgs', mycs, froms', sents, cur_n, @Recv t pat)
+  (* | HonestRecvDrop : forall {A B} {t} (usrs : honest_users A) (adv : user_data B) cs suid gks ks qmsgs qmsgs' *)
+  (*                    mycs froms froms' sents cur_n (msg : crypto t) pat msgs, *)
+  (*     qmsgs = (existT _ _ msg) :: msgs (* we have a message waiting for us! *) *)
+  (*     -> qmsgs' = msgs *)
+  (*     -> froms' = (if msg_signed_addressed (findUserKeys usrs) cs suid msg *)
+  (*                 then updateTrackedNonce suid froms cs msg *)
+  (*                 else froms) *)
+  (*     -> ~ msg_accepted_by_pattern cs suid pat msg *)
+  (*     -> honest_party_step Silent suid (* Error label ... *) *)
+  (*                 (usrs, adv, cs, gks, ks, qmsgs , mycs, froms,  sents, cur_n, Recv pat) *)
+  (*                 (usrs, adv, cs, gks, ks, qmsgs', mycs, froms', sents, cur_n, @Recv t pat) *)
 
-  (* Augment attacker's keys with those available through messages sent, *)
-  (*  * including traversing through ciphers already known by attacker, etc. *)
-  (*  *)
-  | HonestSend : forall {A B} {t} (usrs usrs' : honest_users A) (adv adv' : user_data B)
-                 cs suid gks ks qmsgs mycs froms sents sents' cur_n rec_u_id rec_u newkeys (msg : crypto t),
-      findKeysCrypto cs msg = newkeys
-      -> keys_mine ks newkeys
-      -> incl (findCiphers msg) mycs
-      -> usrs $? rec_u_id = Some rec_u
-      -> Some rec_u_id <> suid
-      -> sents' = updateTrackedNonce (Some rec_u_id) sents cs msg
-      -> usrs' = usrs $+ (rec_u_id, {| key_heap  := rec_u.(key_heap)
-                                      ; protocol  := rec_u.(protocol)
-                                      ; msg_heap  := rec_u.(msg_heap) ++ [existT _ _ msg]
-                                      ; c_heap    := rec_u.(c_heap)
-                                      ; from_nons := rec_u.(from_nons)
-                                      ; sent_nons := rec_u.(sent_nons)
-                                      ; cur_nonce := rec_u.(cur_nonce) |})
-      -> adv' = 
-        {| key_heap  := adv.(key_heap) $k++ newkeys
-           ; protocol  := adv.(protocol)
-           ; msg_heap  := adv.(msg_heap) ++ [existT _ _ msg]
-           ; c_heap    := adv.(c_heap)
-           ; from_nons := adv.(from_nons)
-           ; sent_nons := adv.(sent_nons)
-           ; cur_nonce := adv.(cur_nonce) |}
-      -> honest_party_step (Action (Output msg suid (Some rec_u_id) sents)) suid
-                  (usrs , adv , cs, gks, ks, qmsgs, mycs, froms, sents,  cur_n, Send rec_u_id msg)
-                  (usrs', adv', cs, gks, ks, qmsgs, mycs, froms, sents', cur_n, Return tt)
+  (* (* Augment attacker's keys with those available through messages sent, *) *)
+  (* (*  * including traversing through ciphers already known by attacker, etc. *) *)
+  (* (*  *) *)
+  (* | HonestSend : forall {A B} {t} (usrs usrs' : honest_users A) (adv adv' : user_data B) *)
+  (*                cs suid gks ks qmsgs mycs froms sents sents' cur_n rec_u_id rec_u newkeys (msg : crypto t), *)
+  (*     findKeysCrypto cs msg = newkeys *)
+  (*     -> keys_mine ks newkeys *)
+  (*     -> incl (findCiphers msg) mycs *)
+  (*     -> usrs $? rec_u_id = Some rec_u *)
+  (*     -> Some rec_u_id <> suid *)
+  (*     -> sents' = updateTrackedNonce (Some rec_u_id) sents cs msg *)
+  (*     -> usrs' = usrs $+ (rec_u_id, {| key_heap  := rec_u.(key_heap) *)
+  (*                                     ; protocol  := rec_u.(protocol) *)
+  (*                                     ; msg_heap  := rec_u.(msg_heap) ++ [existT _ _ msg] *)
+  (*                                     ; c_heap    := rec_u.(c_heap) *)
+  (*                                     ; from_nons := rec_u.(from_nons) *)
+  (*                                     ; sent_nons := rec_u.(sent_nons) *)
+  (*                                     ; cur_nonce := rec_u.(cur_nonce) |}) *)
+  (*     -> adv' =  *)
+  (*       {| key_heap  := adv.(key_heap) $k++ newkeys *)
+  (*          ; protocol  := adv.(protocol) *)
+  (*          ; msg_heap  := adv.(msg_heap) ++ [existT _ _ msg] *)
+  (*          ; c_heap    := adv.(c_heap) *)
+  (*          ; from_nons := adv.(from_nons) *)
+  (*          ; sent_nons := adv.(sent_nons) *)
+  (*          ; cur_nonce := adv.(cur_nonce) |} *)
+  (*     -> honest_party_step (Action (Output msg suid (Some rec_u_id) sents)) suid *)
+  (*                 (usrs , adv , cs, gks, ks, qmsgs, mycs, froms, sents,  cur_n, Send rec_u_id msg) *)
+  (*                 (usrs', adv', cs, gks, ks, qmsgs, mycs, froms, sents', cur_n, Return tt) *)
 
-  (* Encryption / Decryption *)
-  | HonestEncrypt : forall {A B} {t} (usrs : honest_users A) (adv : user_data B) cs cs' u_id gks ks qmsgs mycs mycs' froms sents
-                    cur_n cur_n' (msg : message t) k__signid k__encid kp__enc kt__enc kt__sign c_id cipherMsg msg_to,
-      gks $? k__encid  = Some (MkCryptoKey k__encid Encryption kt__enc)
-      -> gks $? k__signid = Some (MkCryptoKey k__signid Signing kt__sign)
-      -> ks $? k__encid   = Some kp__enc
-      -> ks $? k__signid  = Some true
-      -> ~ In c_id cs
-      -> keys_mine ks (findKeysMessage msg)
-      -> cur_n' = 1 + cur_n
-      -> cipherMsg = SigEncCipher k__signid k__encid msg_to (u_id, cur_n) msg
-      -> cs' = cs $+ (c_id, cipherMsg)
-      -> mycs' = c_id :: mycs
-      (* Extra condition *)
-      -> findUserKeys usrs $? k__encid = Some true
-      -> honest_party_step Silent u_id
-                  (usrs, adv, cs , gks, ks, qmsgs, mycs,  froms, sents, cur_n,  SignEncrypt k__signid k__encid msg_to msg)
-                  (usrs, adv, cs', gks, ks, qmsgs, mycs', froms, sents, cur_n', Return (SignedCiphertext c_id))
+  (* (* Encryption / Decryption *) *)
+  (* | HonestEncrypt : forall {A B} {t} (usrs : honest_users A) (adv : user_data B) cs cs' u_id gks ks qmsgs mycs mycs' froms sents *)
+  (*                   cur_n cur_n' (msg : message t) k__signid k__encid kp__enc kt__enc kt__sign c_id cipherMsg msg_to, *)
+  (*     gks $? k__encid  = Some (MkCryptoKey k__encid Encryption kt__enc) *)
+  (*     -> gks $? k__signid = Some (MkCryptoKey k__signid Signing kt__sign) *)
+  (*     -> ks $? k__encid   = Some kp__enc *)
+  (*     -> ks $? k__signid  = Some true *)
+  (*     -> ~ In c_id cs *)
+  (*     -> keys_mine ks (findKeysMessage msg) *)
+  (*     -> cur_n' = 1 + cur_n *)
+  (*     -> cipherMsg = SigEncCipher k__signid k__encid msg_to (u_id, cur_n) msg *)
+  (*     -> cs' = cs $+ (c_id, cipherMsg) *)
+  (*     -> mycs' = c_id :: mycs *)
+  (*     (* Extra condition *) *)
+  (*     -> findUserKeys usrs $? k__encid = Some true *)
+  (*     -> honest_party_step Silent u_id *)
+  (*                 (usrs, adv, cs , gks, ks, qmsgs, mycs,  froms, sents, cur_n,  SignEncrypt k__signid k__encid msg_to msg) *)
+  (*                 (usrs, adv, cs', gks, ks, qmsgs, mycs', froms, sents, cur_n', Return (SignedCiphertext c_id)) *)
 
-  | HonestDecrypt : forall {A B} {t} (usrs : honest_users A) (adv : user_data B) cs u_id gks ks ks' qmsgs mycs mycs'
-                    (msg : message t) k__signid kp__sign k__encid c_id nonce newkeys kt__sign kt__enc msg_to froms sents cur_n,
-      cs $? c_id     = Some (SigEncCipher k__signid k__encid msg_to nonce msg)
-      -> gks $? k__encid  = Some (MkCryptoKey k__encid Encryption kt__enc)
-      -> gks $? k__signid = Some (MkCryptoKey k__signid Signing kt__sign)
-      -> ks  $? k__encid  = Some true
-      -> ks  $? k__signid = Some kp__sign
-      -> findKeysMessage msg = newkeys
-      -> ks' = ks $k++ newkeys
-      -> mycs' = (* newcs ++  *)mycs
-      -> List.In c_id mycs
-      -> honest_party_step Silent u_id
-                  (usrs, adv, cs, gks, ks , qmsgs, mycs,  froms, sents, cur_n, Decrypt (SignedCiphertext c_id))
-                  (usrs, adv, cs, gks, ks', qmsgs, mycs', froms, sents, cur_n, Return msg)
+  (* | HonestDecrypt : forall {A B} {t} (usrs : honest_users A) (adv : user_data B) cs u_id gks ks ks' qmsgs mycs mycs' *)
+  (*                   (msg : message t) k__signid kp__sign k__encid c_id nonce newkeys kt__sign kt__enc msg_to froms sents cur_n, *)
+  (*     cs $? c_id     = Some (SigEncCipher k__signid k__encid msg_to nonce msg) *)
+  (*     -> gks $? k__encid  = Some (MkCryptoKey k__encid Encryption kt__enc) *)
+  (*     -> gks $? k__signid = Some (MkCryptoKey k__signid Signing kt__sign) *)
+  (*     -> ks  $? k__encid  = Some true *)
+  (*     -> ks  $? k__signid = Some kp__sign *)
+  (*     -> findKeysMessage msg = newkeys *)
+  (*     -> ks' = ks $k++ newkeys *)
+  (*     -> mycs' = (* newcs ++  *)mycs *)
+  (*     -> List.In c_id mycs *)
+  (*     -> honest_party_step Silent u_id *)
+  (*                 (usrs, adv, cs, gks, ks , qmsgs, mycs,  froms, sents, cur_n, Decrypt (SignedCiphertext c_id)) *)
+  (*                 (usrs, adv, cs, gks, ks', qmsgs, mycs', froms, sents, cur_n, Return msg) *)
 
-  (* Signing / Verification *)
-  | HonestSign : forall {A B} {t} (usrs : honest_users A) (adv : user_data B) cs cs' u_id gks ks qmsgs mycs mycs' froms sents cur_n cur_n'
-                 (msg : message t) k_id kt c_id cipherMsg msg_to,
-      gks $? k_id = Some (MkCryptoKey k_id Signing kt)
-      -> ks  $? k_id = Some true
-      -> ~ In c_id cs
-      -> cur_n' = 1 + cur_n
-      -> cipherMsg = SigCipher k_id msg_to (u_id, cur_n) msg
-      -> cs' = cs $+ (c_id, cipherMsg)
-      -> mycs' = c_id :: mycs
-      -> honest_party_step Silent u_id
-                  (usrs, adv, cs , gks, ks, qmsgs, mycs,  froms, sents, cur_n,  Sign k_id msg_to msg)
-                  (usrs, adv, cs', gks, ks, qmsgs, mycs', froms, sents, cur_n', Return (SignedCiphertext c_id))
+  (* (* Signing / Verification *) *)
+  (* | HonestSign : forall {A B} {t} (usrs : honest_users A) (adv : user_data B) cs cs' u_id gks ks qmsgs mycs mycs' froms sents cur_n cur_n' *)
+  (*                (msg : message t) k_id kt c_id cipherMsg msg_to, *)
+  (*     gks $? k_id = Some (MkCryptoKey k_id Signing kt) *)
+  (*     -> ks  $? k_id = Some true *)
+  (*     -> ~ In c_id cs *)
+  (*     -> cur_n' = 1 + cur_n *)
+  (*     -> cipherMsg = SigCipher k_id msg_to (u_id, cur_n) msg *)
+  (*     -> cs' = cs $+ (c_id, cipherMsg) *)
+  (*     -> mycs' = c_id :: mycs *)
+  (*     -> honest_party_step Silent u_id *)
+  (*                 (usrs, adv, cs , gks, ks, qmsgs, mycs,  froms, sents, cur_n,  Sign k_id msg_to msg) *)
+  (*                 (usrs, adv, cs', gks, ks, qmsgs, mycs', froms, sents, cur_n', Return (SignedCiphertext c_id)) *)
 
-  | HonestVerify : forall {A B} {t} (usrs : honest_users A) (adv : user_data B) cs u_id gks ks qmsgs mycs froms sents cur_n
-                   (msg : message t) k_id kp kt c_id nonce msg_to,
-      gks $? k_id = Some (MkCryptoKey k_id Signing kt)
-      -> ks  $? k_id = Some kp
-      -> cs $? c_id = Some (SigCipher k_id msg_to nonce msg)
-      -> List.In c_id mycs
-      -> honest_party_step Silent u_id
-                  (usrs, adv, cs, gks, ks, qmsgs, mycs, froms, sents, cur_n, Verify k_id (SignedCiphertext c_id))
-                  (usrs, adv, cs, gks, ks, qmsgs, mycs, froms, sents, cur_n, Return (true, msg))
-  | HonestGenerateSymKey: forall {A B} (usrs : honest_users A) (adv : user_data B)
-                          cs u_id gks gks' ks ks' qmsgs mycs froms sents cur_n
-                          (k_id : key_identifier) k usage,
-      gks $? k_id = None
-      -> k = MkCryptoKey k_id usage SymKey
-      -> gks' = gks $+ (k_id, k)
-      -> ks' = add_key_perm k_id true ks
-      -> honest_party_step Silent u_id
-                  (usrs, adv, cs, gks, ks, qmsgs, mycs, froms, sents, cur_n, GenerateSymKey usage)
-                  (usrs, adv, cs, gks', ks', qmsgs, mycs, froms, sents, cur_n, Return (k_id, true))
-  | HonestGenerateAsymKey: forall {A B} (usrs : honest_users A) (adv : user_data B)
-                           cs u_id gks gks' ks ks' qmsgs mycs froms sents cur_n
-                           (k_id : key_identifier) k usage,
-      gks $? k_id = None
-      -> k = MkCryptoKey k_id usage AsymKey
-      -> gks' = gks $+ (k_id, k)
-      -> ks' = add_key_perm k_id true ks
-      -> honest_party_step Silent u_id
-                  (usrs, adv, cs, gks, ks, qmsgs, mycs, froms, sents, cur_n, GenerateAsymKey usage)
-                  (usrs, adv, cs, gks', ks', qmsgs, mycs, froms, sents, cur_n, Return (k_id, true))
-  .
+  (* | HonestVerify : forall {A B} {t} (usrs : honest_users A) (adv : user_data B) cs u_id gks ks qmsgs mycs froms sents cur_n *)
+  (*                  (msg : message t) k_id kp kt c_id nonce msg_to, *)
+  (*     gks $? k_id = Some (MkCryptoKey k_id Signing kt) *)
+  (*     -> ks  $? k_id = Some kp *)
+  (*     -> cs $? c_id = Some (SigCipher k_id msg_to nonce msg) *)
+  (*     -> List.In c_id mycs *)
+  (*     -> honest_party_step Silent u_id *)
+  (*                 (usrs, adv, cs, gks, ks, qmsgs, mycs, froms, sents, cur_n, Verify k_id (SignedCiphertext c_id)) *)
+  (*                 (usrs, adv, cs, gks, ks, qmsgs, mycs, froms, sents, cur_n, Return (true, msg)) *)
+  (* | HonestGenerateSymKey: forall {A B} (usrs : honest_users A) (adv : user_data B) *)
+  (*                         cs u_id gks gks' ks ks' qmsgs mycs froms sents cur_n *)
+  (*                         (k_id : key_identifier) k usage, *)
+  (*     gks $? k_id = None *)
+  (*     -> k = MkCryptoKey k_id usage SymKey *)
+  (*     -> gks' = gks $+ (k_id, k) *)
+  (*     -> ks' = add_key_perm k_id true ks *)
+  (*     -> honest_party_step Silent u_id *)
+  (*                 (usrs, adv, cs, gks, ks, qmsgs, mycs, froms, sents, cur_n, GenerateSymKey usage) *)
+  (*                 (usrs, adv, cs, gks', ks', qmsgs, mycs, froms, sents, cur_n, Return (k_id, true)) *)
+  (* | HonestGenerateAsymKey: forall {A B} (usrs : honest_users A) (adv : user_data B) *)
+  (*                          cs u_id gks gks' ks ks' qmsgs mycs froms sents cur_n *)
+  (*                          (k_id : key_identifier) k usage, *)
+  (*     gks $? k_id = None *)
+  (*     -> k = MkCryptoKey k_id usage AsymKey *)
+  (*     -> gks' = gks $+ (k_id, k) *)
+  (*     -> ks' = add_key_perm k_id true ks *)
+  (*     -> honest_party_step Silent u_id *)
+  (*                 (usrs, adv, cs, gks, ks, qmsgs, mycs, froms, sents, cur_n, GenerateAsymKey usage) *)
+  (*                 (usrs, adv, cs, gks', ks', qmsgs, mycs, froms, sents, cur_n, Return (k_id, true)) *)
+  (* . *)
 
-  Inductive honest_party_universe_step {A B} : universe A B -> rlabel -> universe A B -> Prop :=
-  | HonestUser  : forall U U' (u_id : user_id) userData usrs adv
-                    cs gks ks qmsgs mycs froms sents cur_n lbl (cmd : user_cmd A),
-      U.(users) $? u_id = Some userData
-      -> honest_party_step
-          lbl (Some u_id)
-          (build_data_step U userData)
-          (usrs, adv, cs, gks, ks, qmsgs, mycs, froms, sents, cur_n, cmd)
-      -> U' = buildUniverse usrs adv cs gks u_id {| key_heap  := ks
-                                                 ; msg_heap  := qmsgs
-                                                 ; protocol  := cmd
-                                                 ; c_heap    := mycs
-                                                 ; from_nons := froms
-                                                 ; sent_nons := sents
-                                                 ; cur_nonce := cur_n |}
-      -> honest_party_universe_step U lbl U'.
-
+  (* Inductive honest_party_universe_step {A B} : universe A B -> rlabel -> universe A B -> Prop := *)
+  (* | HonestUser  : forall U U' (u_id : user_id) userData usrs adv *)
+  (*                   cs gks ks qmsgs mycs froms sents cur_n lbl (cmd : user_cmd A), *)
+  (*     U.(users) $? u_id = Some userData *)
+  (*     -> honest_party_step *)
+  (*         lbl (Some u_id) *)
+  (*         (build_data_step U userData) *)
+  (*         (usrs, adv, cs, gks, ks, qmsgs, mycs, froms, sents, cur_n, cmd) *)
+  (*     -> U' = buildUniverse usrs adv cs gks u_id {| key_heap  := ks *)
+  (*                                                ; msg_heap  := qmsgs *)
+  (*                                                ; protocol  := cmd *)
+  (*                                                ; c_heap    := mycs *)
+  (*                                                ; from_nons := froms *)
+  (*                                                ; sent_nons := sents *)
+  (*                                                ; cur_nonce := cur_n |} *)
+  (*     -> honest_party_universe_step U lbl U'. *)
 
 End OperationalSemanticsPredicates.
 
@@ -462,16 +461,15 @@ Section Simulation.
         /\ action_matches a1 U__r a2 U__i'
         /\ R (RealWorld.peel_adv U__r') U__i''.
 
-  Definition simulates_universe_ok' :=
-    forall (U__r : RealWorld.universe A B) U__i,
-        R (RealWorld.peel_adv U__r) U__i
-      -> universe_ok U__r
-      -> adv_universe_ok U__r
-      -> advP U__r.(RealWorld.adversary)
-      -> forall U__r' lbl,
-            RealWorld.step_universe U__r lbl U__r'
-          -> honest_party_universe_step U__r lbl U__r'.
-          (* \/ U__r.(RealWorld.all_ciphers) = U__r'.(RealWorld.all_ciphers). *)
+  (* Definition simulates_universe_ok' := *)
+  (*   forall (U__r : RealWorld.universe A B) U__i, *)
+  (*       R (RealWorld.peel_adv U__r) U__i *)
+  (*     -> universe_ok U__r *)
+  (*     -> adv_universe_ok U__r *)
+  (*     -> advP U__r.(RealWorld.adversary) *)
+  (*     -> forall U__r' lbl, *)
+  (*           RealWorld.step_universe U__r lbl U__r' *)
+  (*         -> honest_party_universe_step U__r lbl U__r'. *)
 
   Definition simulates_universe_ok :=
     forall B (U__r : RealWorld.universe A B) U__i,
